---
title: Causality.Relation.Binary.PropositionalEquality.≡-Reasoning
---

Definitions and proofs to help with reasoning about propositional equality.

<pre class="Agda"><a id="162" class="Symbol">{-#</a> <a id="166" class="Keyword">OPTIONS</a> <a id="174" class="Pragma">--without-K</a> <a id="186" class="Pragma">--safe</a> <a id="193" class="Symbol">#-}</a>

<a id="198" class="Keyword">module</a> <a id="205" href="Causality.Relation.Binary.PropositionalEquality.%25E2%2589%25A1-Reasoning.html" class="Module">Causality.Relation.Binary.PropositionalEquality.≡-Reasoning</a> <a id="265" class="Symbol">{</a><a id="266" href="Causality.Relation.Binary.PropositionalEquality.%25E2%2589%25A1-Reasoning.html#266" class="Bound">a</a><a id="267" class="Symbol">}</a> <a id="269" class="Symbol">{</a><a id="270" href="Causality.Relation.Binary.PropositionalEquality.%25E2%2589%25A1-Reasoning.html#270" class="Bound">A</a> <a id="272" class="Symbol">:</a> <a id="274" href="Agda.Primitive.html#320" class="Primitive">Set</a> <a id="278" href="Causality.Relation.Binary.PropositionalEquality.%25E2%2589%25A1-Reasoning.html#266" class="Bound">a</a><a id="279" class="Symbol">}</a> <a id="281" class="Keyword">where</a>

<a id="288" class="Keyword">open</a> <a id="293" class="Keyword">import</a> <a id="300" href="Relation.Binary.PropositionalEquality.html" class="Module">Relation.Binary.PropositionalEquality</a> <a id="338" class="Keyword">using</a> <a id="344" class="Symbol">(</a><a id="345" href="Agda.Builtin.Equality.html#133" class="Datatype Operator">_≡_</a><a id="348" class="Symbol">;</a> <a id="350" href="Agda.Builtin.Equality.html#190" class="InductiveConstructor">refl</a><a id="354" class="Symbol">;</a> <a id="356" href="Relation.Binary.PropositionalEquality.Core.html#1707" class="Function">sym</a><a id="359" class="Symbol">;</a> <a id="361" href="Relation.Binary.PropositionalEquality.Core.html#1752" class="Function">trans</a><a id="366" class="Symbol">)</a>

<a id="369" class="Keyword">infix</a>  <a id="376" class="Number">3</a> <a id="378" href="Causality.Relation.Binary.PropositionalEquality.%25E2%2589%25A1-Reasoning.html#767" class="Function Operator">_∎</a>
<a id="381" class="Keyword">infixr</a> <a id="388" class="Number">2</a> <a id="390" href="Causality.Relation.Binary.PropositionalEquality.%25E2%2589%25A1-Reasoning.html#483" class="Function Operator">_≡⟨⟩_</a> <a id="396" href="Causality.Relation.Binary.PropositionalEquality.%25E2%2589%25A1-Reasoning.html#536" class="Function Operator">_≡⟨_⟩_</a> <a id="403" href="Causality.Relation.Binary.PropositionalEquality.%25E2%2589%25A1-Reasoning.html#615" class="Function Operator">_≡⟨_⟩⟨_⟩_</a>
<a id="413" class="Keyword">infix</a>  <a id="420" class="Number">1</a> <a id="422" href="Causality.Relation.Binary.PropositionalEquality.%25E2%2589%25A1-Reasoning.html#430" class="Function Operator">begin_</a>

<a id="begin_"></a><a id="430" href="Causality.Relation.Binary.PropositionalEquality.%25E2%2589%25A1-Reasoning.html#430" class="Function Operator">begin_</a> <a id="437" class="Symbol">:</a> <a id="439" class="Symbol">{</a><a id="440" href="Causality.Relation.Binary.PropositionalEquality.%25E2%2589%25A1-Reasoning.html#440" class="Bound">x</a> <a id="442" href="Causality.Relation.Binary.PropositionalEquality.%25E2%2589%25A1-Reasoning.html#442" class="Bound">y</a> <a id="444" class="Symbol">:</a> <a id="446" href="Causality.Relation.Binary.PropositionalEquality.%25E2%2589%25A1-Reasoning.html#270" class="Bound">A</a><a id="447" class="Symbol">}</a> <a id="449" class="Symbol">→</a> <a id="451" href="Causality.Relation.Binary.PropositionalEquality.%25E2%2589%25A1-Reasoning.html#440" class="Bound">x</a> <a id="453" href="Agda.Builtin.Equality.html#133" class="Datatype Operator">≡</a> <a id="455" href="Causality.Relation.Binary.PropositionalEquality.%25E2%2589%25A1-Reasoning.html#442" class="Bound">y</a> <a id="457" class="Symbol">→</a> <a id="459" href="Causality.Relation.Binary.PropositionalEquality.%25E2%2589%25A1-Reasoning.html#440" class="Bound">x</a> <a id="461" href="Agda.Builtin.Equality.html#133" class="Datatype Operator">≡</a> <a id="463" href="Causality.Relation.Binary.PropositionalEquality.%25E2%2589%25A1-Reasoning.html#442" class="Bound">y</a>
<a id="465" href="Causality.Relation.Binary.PropositionalEquality.%25E2%2589%25A1-Reasoning.html#430" class="Function Operator">begin_</a> <a id="472" href="Causality.Relation.Binary.PropositionalEquality.%25E2%2589%25A1-Reasoning.html#472" class="Bound">x≡y</a> <a id="476" class="Symbol">=</a> <a id="478" href="Causality.Relation.Binary.PropositionalEquality.%25E2%2589%25A1-Reasoning.html#472" class="Bound">x≡y</a>

<a id="_≡⟨⟩_"></a><a id="483" href="Causality.Relation.Binary.PropositionalEquality.%25E2%2589%25A1-Reasoning.html#483" class="Function Operator">_≡⟨⟩_</a> <a id="489" class="Symbol">:</a> <a id="491" class="Symbol">(</a><a id="492" href="Causality.Relation.Binary.PropositionalEquality.%25E2%2589%25A1-Reasoning.html#492" class="Bound">x</a> <a id="494" class="Symbol">{</a><a id="495" href="Causality.Relation.Binary.PropositionalEquality.%25E2%2589%25A1-Reasoning.html#495" class="Bound">y</a><a id="496" class="Symbol">}</a> <a id="498" class="Symbol">:</a> <a id="500" href="Causality.Relation.Binary.PropositionalEquality.%25E2%2589%25A1-Reasoning.html#270" class="Bound">A</a><a id="501" class="Symbol">)</a> <a id="503" class="Symbol">→</a> <a id="505" href="Causality.Relation.Binary.PropositionalEquality.%25E2%2589%25A1-Reasoning.html#492" class="Bound">x</a> <a id="507" href="Agda.Builtin.Equality.html#133" class="Datatype Operator">≡</a> <a id="509" href="Causality.Relation.Binary.PropositionalEquality.%25E2%2589%25A1-Reasoning.html#495" class="Bound">y</a> <a id="511" class="Symbol">→</a> <a id="513" href="Causality.Relation.Binary.PropositionalEquality.%25E2%2589%25A1-Reasoning.html#492" class="Bound">x</a> <a id="515" href="Agda.Builtin.Equality.html#133" class="Datatype Operator">≡</a> <a id="517" href="Causality.Relation.Binary.PropositionalEquality.%25E2%2589%25A1-Reasoning.html#495" class="Bound">y</a>
<a id="519" class="Symbol">_</a> <a id="521" href="Causality.Relation.Binary.PropositionalEquality.%25E2%2589%25A1-Reasoning.html#483" class="Function Operator">≡⟨⟩</a> <a id="525" href="Causality.Relation.Binary.PropositionalEquality.%25E2%2589%25A1-Reasoning.html#525" class="Bound">x≡y</a> <a id="529" class="Symbol">=</a> <a id="531" href="Causality.Relation.Binary.PropositionalEquality.%25E2%2589%25A1-Reasoning.html#525" class="Bound">x≡y</a>

<a id="_≡⟨_⟩_"></a><a id="536" href="Causality.Relation.Binary.PropositionalEquality.%25E2%2589%25A1-Reasoning.html#536" class="Function Operator">_≡⟨_⟩_</a> <a id="543" class="Symbol">:</a> <a id="545" class="Symbol">(</a><a id="546" href="Causality.Relation.Binary.PropositionalEquality.%25E2%2589%25A1-Reasoning.html#546" class="Bound">x</a> <a id="548" class="Symbol">{</a><a id="549" href="Causality.Relation.Binary.PropositionalEquality.%25E2%2589%25A1-Reasoning.html#549" class="Bound">y</a> <a id="551" href="Causality.Relation.Binary.PropositionalEquality.%25E2%2589%25A1-Reasoning.html#551" class="Bound">z</a><a id="552" class="Symbol">}</a> <a id="554" class="Symbol">:</a> <a id="556" href="Causality.Relation.Binary.PropositionalEquality.%25E2%2589%25A1-Reasoning.html#270" class="Bound">A</a><a id="557" class="Symbol">)</a> <a id="559" class="Symbol">→</a> <a id="561" href="Causality.Relation.Binary.PropositionalEquality.%25E2%2589%25A1-Reasoning.html#546" class="Bound">x</a> <a id="563" href="Agda.Builtin.Equality.html#133" class="Datatype Operator">≡</a> <a id="565" href="Causality.Relation.Binary.PropositionalEquality.%25E2%2589%25A1-Reasoning.html#549" class="Bound">y</a> <a id="567" class="Symbol">→</a> <a id="569" href="Causality.Relation.Binary.PropositionalEquality.%25E2%2589%25A1-Reasoning.html#549" class="Bound">y</a> <a id="571" href="Agda.Builtin.Equality.html#133" class="Datatype Operator">≡</a> <a id="573" href="Causality.Relation.Binary.PropositionalEquality.%25E2%2589%25A1-Reasoning.html#551" class="Bound">z</a> <a id="575" class="Symbol">→</a> <a id="577" href="Causality.Relation.Binary.PropositionalEquality.%25E2%2589%25A1-Reasoning.html#546" class="Bound">x</a> <a id="579" href="Agda.Builtin.Equality.html#133" class="Datatype Operator">≡</a> <a id="581" href="Causality.Relation.Binary.PropositionalEquality.%25E2%2589%25A1-Reasoning.html#551" class="Bound">z</a>
<a id="583" class="Symbol">_</a> <a id="585" href="Causality.Relation.Binary.PropositionalEquality.%25E2%2589%25A1-Reasoning.html#536" class="Function Operator">≡⟨</a> <a id="588" href="Causality.Relation.Binary.PropositionalEquality.%25E2%2589%25A1-Reasoning.html#588" class="Bound">x≡y</a> <a id="592" href="Causality.Relation.Binary.PropositionalEquality.%25E2%2589%25A1-Reasoning.html#536" class="Function Operator">⟩</a> <a id="594" href="Causality.Relation.Binary.PropositionalEquality.%25E2%2589%25A1-Reasoning.html#594" class="Bound">y≡z</a> <a id="598" class="Symbol">=</a> <a id="600" href="Relation.Binary.PropositionalEquality.Core.html#1752" class="Function">trans</a> <a id="606" href="Causality.Relation.Binary.PropositionalEquality.%25E2%2589%25A1-Reasoning.html#588" class="Bound">x≡y</a> <a id="610" href="Causality.Relation.Binary.PropositionalEquality.%25E2%2589%25A1-Reasoning.html#594" class="Bound">y≡z</a>

<a id="_≡⟨_⟩⟨_⟩_"></a><a id="615" href="Causality.Relation.Binary.PropositionalEquality.%25E2%2589%25A1-Reasoning.html#615" class="Function Operator">_≡⟨_⟩⟨_⟩_</a> <a id="625" class="Symbol">:</a> <a id="627" class="Symbol">∀</a> <a id="629" class="Symbol">{</a><a id="630" href="Causality.Relation.Binary.PropositionalEquality.%25E2%2589%25A1-Reasoning.html#630" class="Bound">b</a><a id="631" class="Symbol">}</a> <a id="633" class="Symbol">{</a><a id="634" href="Causality.Relation.Binary.PropositionalEquality.%25E2%2589%25A1-Reasoning.html#634" class="Bound">B</a> <a id="636" class="Symbol">:</a> <a id="638" href="Agda.Primitive.html#320" class="Primitive">Set</a> <a id="642" href="Causality.Relation.Binary.PropositionalEquality.%25E2%2589%25A1-Reasoning.html#630" class="Bound">b</a><a id="643" class="Symbol">}</a> <a id="645" class="Symbol">(</a><a id="646" href="Causality.Relation.Binary.PropositionalEquality.%25E2%2589%25A1-Reasoning.html#646" class="Bound">x</a> <a id="648" class="Symbol">{</a><a id="649" href="Causality.Relation.Binary.PropositionalEquality.%25E2%2589%25A1-Reasoning.html#649" class="Bound">y</a> <a id="651" href="Causality.Relation.Binary.PropositionalEquality.%25E2%2589%25A1-Reasoning.html#651" class="Bound">z</a><a id="652" class="Symbol">}</a> <a id="654" class="Symbol">:</a> <a id="656" href="Causality.Relation.Binary.PropositionalEquality.%25E2%2589%25A1-Reasoning.html#270" class="Bound">A</a><a id="657" class="Symbol">)</a> <a id="659" class="Symbol">{</a><a id="660" href="Causality.Relation.Binary.PropositionalEquality.%25E2%2589%25A1-Reasoning.html#660" class="Bound">x′</a> <a id="663" href="Causality.Relation.Binary.PropositionalEquality.%25E2%2589%25A1-Reasoning.html#663" class="Bound">y′</a> <a id="666" class="Symbol">:</a> <a id="668" href="Causality.Relation.Binary.PropositionalEquality.%25E2%2589%25A1-Reasoning.html#634" class="Bound">B</a><a id="669" class="Symbol">}</a> <a id="671" class="Symbol">→</a> <a id="673" href="Causality.Relation.Binary.PropositionalEquality.%25E2%2589%25A1-Reasoning.html#660" class="Bound">x′</a> <a id="676" href="Agda.Builtin.Equality.html#133" class="Datatype Operator">≡</a> <a id="678" href="Causality.Relation.Binary.PropositionalEquality.%25E2%2589%25A1-Reasoning.html#663" class="Bound">y′</a> <a id="681" class="Symbol">→</a> <a id="683" class="Symbol">(</a><a id="684" href="Causality.Relation.Binary.PropositionalEquality.%25E2%2589%25A1-Reasoning.html#660" class="Bound">x′</a> <a id="687" href="Agda.Builtin.Equality.html#133" class="Datatype Operator">≡</a> <a id="689" href="Causality.Relation.Binary.PropositionalEquality.%25E2%2589%25A1-Reasoning.html#663" class="Bound">y′</a> <a id="692" class="Symbol">→</a> <a id="694" href="Causality.Relation.Binary.PropositionalEquality.%25E2%2589%25A1-Reasoning.html#646" class="Bound">x</a> <a id="696" href="Agda.Builtin.Equality.html#133" class="Datatype Operator">≡</a> <a id="698" href="Causality.Relation.Binary.PropositionalEquality.%25E2%2589%25A1-Reasoning.html#649" class="Bound">y</a><a id="699" class="Symbol">)</a> <a id="701" class="Symbol">→</a> <a id="703" href="Causality.Relation.Binary.PropositionalEquality.%25E2%2589%25A1-Reasoning.html#649" class="Bound">y</a> <a id="705" href="Agda.Builtin.Equality.html#133" class="Datatype Operator">≡</a> <a id="707" href="Causality.Relation.Binary.PropositionalEquality.%25E2%2589%25A1-Reasoning.html#651" class="Bound">z</a> <a id="709" class="Symbol">→</a> <a id="711" href="Causality.Relation.Binary.PropositionalEquality.%25E2%2589%25A1-Reasoning.html#646" class="Bound">x</a> <a id="713" href="Agda.Builtin.Equality.html#133" class="Datatype Operator">≡</a> <a id="715" href="Causality.Relation.Binary.PropositionalEquality.%25E2%2589%25A1-Reasoning.html#651" class="Bound">z</a>
<a id="717" href="Causality.Relation.Binary.PropositionalEquality.%25E2%2589%25A1-Reasoning.html#717" class="Bound">x</a> <a id="719" href="Causality.Relation.Binary.PropositionalEquality.%25E2%2589%25A1-Reasoning.html#615" class="Function Operator">≡⟨</a> <a id="722" href="Causality.Relation.Binary.PropositionalEquality.%25E2%2589%25A1-Reasoning.html#722" class="Bound">x′≡y′</a> <a id="728" href="Causality.Relation.Binary.PropositionalEquality.%25E2%2589%25A1-Reasoning.html#615" class="Function Operator">⟩⟨</a> <a id="731" href="Causality.Relation.Binary.PropositionalEquality.%25E2%2589%25A1-Reasoning.html#731" class="Bound">lift</a> <a id="736" href="Causality.Relation.Binary.PropositionalEquality.%25E2%2589%25A1-Reasoning.html#615" class="Function Operator">⟩</a> <a id="738" href="Causality.Relation.Binary.PropositionalEquality.%25E2%2589%25A1-Reasoning.html#738" class="Bound">y≡z</a> <a id="742" class="Symbol">=</a> <a id="744" href="Causality.Relation.Binary.PropositionalEquality.%25E2%2589%25A1-Reasoning.html#717" class="Bound">x</a> <a id="746" href="Causality.Relation.Binary.PropositionalEquality.%25E2%2589%25A1-Reasoning.html#536" class="Function Operator">≡⟨</a> <a id="749" href="Causality.Relation.Binary.PropositionalEquality.%25E2%2589%25A1-Reasoning.html#731" class="Bound">lift</a> <a id="754" href="Causality.Relation.Binary.PropositionalEquality.%25E2%2589%25A1-Reasoning.html#722" class="Bound">x′≡y′</a> <a id="760" href="Causality.Relation.Binary.PropositionalEquality.%25E2%2589%25A1-Reasoning.html#536" class="Function Operator">⟩</a> <a id="762" href="Causality.Relation.Binary.PropositionalEquality.%25E2%2589%25A1-Reasoning.html#738" class="Bound">y≡z</a>

<a id="_∎"></a><a id="767" href="Causality.Relation.Binary.PropositionalEquality.%25E2%2589%25A1-Reasoning.html#767" class="Function Operator">_∎</a> <a id="770" class="Symbol">:</a> <a id="772" class="Symbol">∀</a> <a id="774" class="Symbol">(</a><a id="775" href="Causality.Relation.Binary.PropositionalEquality.%25E2%2589%25A1-Reasoning.html#775" class="Bound">x</a> <a id="777" class="Symbol">:</a> <a id="779" href="Causality.Relation.Binary.PropositionalEquality.%25E2%2589%25A1-Reasoning.html#270" class="Bound">A</a><a id="780" class="Symbol">)</a> <a id="782" class="Symbol">→</a> <a id="784" href="Causality.Relation.Binary.PropositionalEquality.%25E2%2589%25A1-Reasoning.html#775" class="Bound">x</a> <a id="786" href="Agda.Builtin.Equality.html#133" class="Datatype Operator">≡</a> <a id="788" href="Causality.Relation.Binary.PropositionalEquality.%25E2%2589%25A1-Reasoning.html#775" class="Bound">x</a>
<a id="790" href="Causality.Relation.Binary.PropositionalEquality.%25E2%2589%25A1-Reasoning.html#767" class="Function Operator">_∎</a> <a id="793" class="Symbol">_</a> <a id="795" class="Symbol">=</a> <a id="797" href="Agda.Builtin.Equality.html#190" class="InductiveConstructor">refl</a>
</pre>